walkup wip

coq/walkup.v
@@ -1,12 +1,5 @@
 (* (c) Copyright Microsoft Corporation and Inria. All rights reserved. *)
-Require Import ssreflect.
-Require Import ssrbool.
-Require Import funs.
-Require Import dataset.
-Require Import ssrnat.
-Require Import seq.
-Require Import finset.
-Require Import paths.
+Require Import ssreflect ssrfun ssrbool eqtype ssrnat seq fintype path.
 Require Import connect.
 Require Import hypermap.
 
@@ -27,27 +20,27 @@ Section Walkup.
 
 Variables (g : hypermap) (z : g).
 
-Let d' := subFin (setC1 z).
-Let to_d' : forall x, setC1 z x -> d' := @subdI _ _.
-Let to_g : d' -> g := @subdE _ _.
+Let d' := {x | x \in (predC1 z)}.
+Let to_d' : forall x, x \in predC1 z -> d' := @exist _ _.
+Let to_g : d' -> g := sval.
 
-Remark z_to_g : forall u, (z =d to_g u) = false.
-Proof. by move=> [x Hx]; apply negbE. Qed.
+Remark z_to_g : forall u, (z == to_g u) = false.
+Proof. by move=> [x Hx] /=; rewrite /predC1 inE /= eq_sym in Hx; apply negbTE. Qed.
 
-Remark to_g_inj : injective to_g. Proof. apply: subdE_inj. Qed.
+Remark to_g_inj : injective to_g. Proof. apply: val_inj. Qed.
 
 Section Skip.
 
 Variable f : g -> g.
 Hypothesis Hf : injective f.
 
-Definition skip1 x := if z =d f x then f z else f x.
+Definition skip1 x := if z == f x then f z else f x.
 
-Lemma skipP : forall u, setC1 z (skip1 (to_g u)).
+Lemma skipP : forall u, skip1 (to_g u) \in predC1 z.
 Proof.
-move=> [x Hx]; rewrite /skip1 /setC1 /=.
-case Hfx: (eqd z (f x)); last by rewrite Hfx.
-by apply/eqP => [Dfz]; case/idP: Hx; rewrite -(inj_eqd Hf) -Dfz.
+move=> [x Hx]; rewrite /skip1 /predC1 /=.
+case Hfx: (z == (f x)); last by rewrite inE /= eq_sym Hfx.
+by apply/eqP => [Dfz]; case/idP: Hx; rewrite /predC1 inE /= -(inj_eq Hf) Dfz eq_sym Hfx.
 Qed.
 
 Definition skip u := to_d' (skipP u).
@@ -56,22 +49,22 @@ Remark inj_skip : injective skip.
 Proof.
 move=> [x Hx] [y Hy] [Hxy]; apply: to_g_inj; move: Hxy; rewrite /= /skip1.
 case: (z =P f x) => [Dfx|_].
-  rewrite {2}Dfx (inj_eqd Hf); case: (x =P y) => [H|_] //.
-  by move=> Dy; rewrite (Hf Dy) setC11 in Hy.
-case (eqd z (f y)); last by apply Hf.
-by move=> Dx; rewrite (Hf Dx) setC11 in Hx.
+  rewrite {2}Dfx (inj_eq Hf); case: (x =P y) => [H|_] //.
+  by move=> Dy; rewrite (Hf Dy) inE /= eqxx in Hy.
+case (z == (f y)); last by apply Hf.
+by move=> Dx; rewrite (Hf Dx) inE /= eqxx in Hx.
 Qed.
 
 Lemma subdE_skip : forall u v, to_g v = f (to_g u) -> v = skip u.
 Proof.
 move=> [x Hx] [y Hy] /= Dy; apply: to_g_inj.
-by rewrite /= /skip1 -Dy (negbE Hy).
+by rewrite /= /skip1 -Dy /= eq_sym (negbTE Hy).
 Qed.
 
-Lemma base_skip : fun_base to_g f skip (set1 (finv f z)).
+Lemma base_skip : fun_base to_g f skip (pred1 (finv f z)).
 Proof.
-move=> [x Hx] y'; rewrite /eqdf {3}/eqd /= /skip1.
-by rewrite (monic2F_eqd (f_finv Hf)); move/negbE=> ->.
+move=> [x Hx] y'. rewrite /frel /= -(inj_eq val_inj) /= /skip1.
+by rewrite eq_sym (monic2F_eqd (f_finv Hf)); move/negbTE=> ->.
 Qed.
 
 Lemma fconnect_skip : forall u v, fconnect skip u v = fconnect f (to_g u) (to_g v).
@@ -85,70 +78,72 @@ move=> u v; apply/idP/idP; move/connectP=> [p Hp Ep].
 elim: {p}(S (size p)) {-2}p u (ltnSn (size p)) Hp Ep => [|n Hrec] // [|y p] u /=.
   by move=> _ _ Dv; apply eq_connect0; apply: to_g_inj.
 move=> Hn; move/andP=> [Dy Hp] Ep.
-case Hy: (setC1 z y).
+case Hy: (predC1 z y).
   apply: (connect_trans (connect1 _) (Hrec p (to_d' Hy) Hn Hp Ep)).
-  by rewrite /eqdf /= /eqd /= /skip1 (eqP Dy) (negbE Hy) set11.
-case: p Hn Hp Ep => [|fy p] Hn /= Hp Ep; first by rewrite /setC1 Ep z_to_g in Hy.
-have Hfy: setC1 z (f y).
-  rewrite /setC1 (eqP (negbEf Hy)) -{1}(eqP Dy) (inj_eqd Hf).
-  by rewrite -(eqP (negbEf Hy)) eqd_sym z_to_g.
+  by rewrite /frel /= -(inj_eq val_inj) /= /skip1 (eqP Dy) [z==y]eq_sym (negbTE Hy) eqxx.
+case: p Hn Hp Ep => [|fy p] Hn /= Hp Ep; first by rewrite /predC1 Ep /= eq_sym z_to_g in Hy.
+have Hfy: predC1 z (f y).
+  rewrite /predC1 /= in Hy.
+  rewrite /predC1 -(eqP (negbFE Hy)) -{1}(eqP Dy) /= (inj_eq Hf).
+  by rewrite (eqP (negbFE Hy)) z_to_g.
 move/andP: Hp => [Dfy Hp]; rewrite (eqP Dfy) in Hfy.
 apply: (connect_trans (connect1 _) (Hrec p (to_d' Hfy) (ltnW Hn) Hp Ep)).
-by rewrite /eqdf /= /eqd /= /skip1 (eqP Dy) (eqP (negbEf Hy)) set11.
+by rewrite /frel /= -(inj_eq val_inj) /= /skip1 (eqP Dy) -(eqP Dfy) (eqP (negbFE Hy)) eqxx.
 Qed.
 
-Lemma fcard_skip : (z =d f z) + fcard skip d' = fcard f g.
+Lemma fcard_skip : (z == f z) + fcard skip {: d'} = fcard f g.
 Proof.
 have Hfg := fconnect_sym Hf; have Hsf := fconnect_sym inj_skip.
 pose a := fconnect f z.
-have Ha: fclosed f (setC a) by apply setC_closed; apply: connect_closed.
-have Haf: fun_adjunction to_g f skip (setC a).
+have Ha: fclosed f (predC a) by apply setC_closed; apply: connect_closed.
+have Haf: fun_adjunction to_g f skip (predC a).
   apply: (strict_adjunction Hsf Ha to_g_inj).
-  apply/subsetP => [x Hax]; case Hx: (z =d x).
-    by rewrite -(eqP Hx) /setC /(a) connect0 in Hax.
-    exact (codom_f _ (to_d' (negbI Hx))).
+  apply/subsetP => [x Hax]; case Hx: (x == z).
+    by rewrite (eqP Hx) /predC /(a) inE /= connect0 in Hax.
+    exact (codom_f _ (to_d' (negbT Hx))).
   move=> u v Hu; apply: base_skip; apply/eqP => /= Du.
-  by rewrite -Du /setC /(a) fconnect_finv in Hu.
-rewrite (n_compC a) (n_compC (preimage to_g a)) {3}/a (n_comp_connect Hfg).
+  by rewrite Du /predC /(a) inE /=  fconnect_finv in Hu.
+rewrite (n_compC a) (n_compC (preim to_g a)) {3}/a (n_comp_connect Hfg).
 rewrite (adjunction_n_comp _ Hfg Hsf Ha Haf) addnA; congr addn.
-case Hfz: (z =d f z).
-  apply: eqP; apply/set0P => [[x Hx]]; apply/andP => [[_ Hzx]].
-  rewrite /preimage /= in Hzx; case/eqP: Hx; move/connectP: Hzx => [p Hp <-] {x}.
+rewrite eq_sym.
+case Hfz: (f z == z).
+  apply: eqP; apply/pred0P => [[x Hx]]; apply/andP => [[_ Hzx]].
+  rewrite /preim /= in Hzx; case/eqP: Hx; move/connectP: Hzx => [p Hp <-] {x}.
   elim: p (z) (eqP Hfz) Hp => [|y p Hrec] x //= Dx; case/andP; case/eqP=> <-.
-  rewrite -(Dx); exact: Hrec Dx.
-apply: etrans (n_comp_connect Hsf (to_d' (negbI Hfz))); apply: eq_n_comp_r.
+  rewrite Dx; exact: Hrec Dx.
+apply: etrans (n_comp_connect Hsf (to_d' (negbT Hfz))); apply: eq_n_comp_r.
 move=> u; apply/idP/idP => Hu.
-  rewrite /preimage /a Hfg in Hu; move/connectP: Hu => [p Hp Dz].
+  rewrite /preim /a inE /= Hfg in Hu; move/connectP: Hu => [p Hp Dz].
   rewrite Hsf; elim: p u Hp Dz => [|x p Hrec] u /=.
     by move=> _ Dz; case/eqP: (z_to_g u); rewrite -Dz.
-  case/andP; move/eqP=> Hx Hp Dz; case Hv: (z =d x).
-    by apply connect1; rewrite /eqdf /eqd /= /skip1 Hx eqd_sym Hv set11.
-  apply: (connect_trans (connect1 _) (Hrec (to_d' (negbI Hv)) Hp Dz)).
-  by rewrite /eqdf /eqd /= /skip1 Hx eqd_sym Hv set11.
+  case/andP; move/eqP=> Hx Hp Dz; case Hv: (x == z).
+    by apply connect1; rewrite /frel /= -(inj_eq val_inj) /= /skip1 Hx eq_sym [z==x]eq_sym Hv eqxx.
+  apply: (connect_trans (connect1 _) (Hrec (to_d' (negbT Hv)) Hp Dz)).
+   by rewrite /frel /= -(inj_eq val_inj) /= /skip1 Hx [z==x]eq_sym Hv eqxx.
 rewrite Hsf in Hu; move/connectP: Hu => [p Hp Dfz].
 elim: p u Hp Dfz => [|v p Hrec] u /=.
-  by move=> _ Du; rewrite Du /preimage /= /a fconnect1.
+  by move=> _ Du; rewrite Du /preim /= /a fconnect1.
 move/andP=> [Huv Hp] Dfz; move: u Huv => [x Hx].
-rewrite /eqdf /eqd /= -/to_g /skip1.
+rewrite /frel -(inj_eq val_inj) /= -/to_g /skip1.
 case: (z =P f x) => [Dz|_] Dfx.
-  by rewrite /preimage /a /= Dz Hfg fconnect1.
+  by rewrite /preim /a /= Dz Hfg fconnect1.
 by apply: (connect_trans (Hrec _ Hp Dfz)); rewrite Hfg; apply connect1.
 Qed.
 
 End Skip.
 
 Definition skip_edge1 x :=
-  if z =d edge z then edge x else
-  if z =d face (edge x) then edge z else
-  if z =d edge x then edge (node z) else edge x.
+  if z == edge z then edge x else
+  if z == face (edge x) then edge z else
+  if z == edge x then edge (node z) else edge x.
 
-Lemma skip_edgeP : forall u, setC1 z (skip_edge1 (to_g u)).
+Lemma skip_edgeP : forall u, predC1 z (skip_edge1 (to_g u)).
 Proof.
-move=> [x Hx]; rewrite /= /skip_edge1 /setC1; case Hez: (z =d edge z).
-  by rewrite (eqP Hez) (inj_eqd (Iedge g)).
-  case Hfex: (z =d face (edge x)); first by rewrite Hez.
-  case Hex: (z =d edge x); last by rewrite Hex.
-by rewrite -(inj_eqd (Iface g)) {1}(eqP Hex) Enode eqd_sym Hfex.
+move=> [x Hx]; rewrite /= /skip_edge1 /predC1; case Hez: (z == edge z).
+  by rewrite (eqP Hez) (inj_eq (Iedge g)).
+  case Hfex: (z == face (edge x)); first by rewrite eq_sym Hez.
+  case Hex: (z == edge x); last by rewrite eq_sym Hex.
+by rewrite -(inj_eq (Iface g)) {2}(eqP Hex) Enode Hfex.
 Qed.
 
 Definition skip_edge u := to_d' (skip_edgeP u).
@@ -156,14 +151,14 @@ Definition skip_edge u := to_d' (skip_edgeP u).
 Lemma Eskip : monic3 skip_edge (skip (Inode g)) (skip (Iface g)).
 Proof.
 move=> [x Hx]; apply: to_g_inj; rewrite /= /skip_edge1 /skip1.
-case Hez: (z =d edge z).
-  case: (z =P face (edge x)) => [Dz|_]; last by rewrite Eedge (negbE Hx).
-  by rewrite {2}(eqP Hez) Eedge set11 Dz Eedge.
-case Hfex: (z =d face (edge x)).
-  rewrite {2 6}(eqP Hfex) (inj_eqd (Iface g)) (inj_eqd (Iedge g)).
-  by rewrite (eqd_sym x) (negbE Hx) !Eedge set11.
-case Hex: (z =d edge x); last by rewrite Hfex Eedge (negbE Hx).
-by rewrite Enode set11 {2 4}(eqP Hex) Eedge (negbE Hx).
+case Hez: (z == edge z).
+  case: (z =P face (edge x)) => [Dz|_]; last by rewrite Eedge [z==x]eq_sym (negbTE Hx).
+  by rewrite {2}(eqP Hez) Eedge eqxx Dz Eedge.
+case Hfex: (z == face (edge x)).
+  rewrite {2 6}(eqP Hfex) (inj_eq (Iface g)) (inj_eq (Iedge g)).
+  by rewrite (eq_sym x) [z==x]eq_sym (negbTE Hx) !Eedge eqxx.
+case Hex: (z == edge x); last by rewrite Hfex Eedge [z==x]eq_sym (negbTE Hx).
+by rewrite Enode eqxx {2 4}(eqP Hex) Eedge [z==x]eq_sym (negbTE Hx).
 Qed.
 
 Definition walkupE := Hypermap Eskip.
@@ -173,24 +168,24 @@ Notation Local g' := walkupE.
 Notation Local "'@' 'g'' H" := ((to_d' H) : g') (at level 10, H at level 8).
 Notation Local "'@' 'g'" := (to_g : g' -> g) (at level 10).
 
-Definition walkupI u x := if subdIopt (setC1 z) x is Some v then v : g' else u.
+Definition walkupI u x := if subdIopt (predC1 z) x is Some v then v : g' else u.
 
-Lemma walkupI_eq : forall u x, @g (walkupI u x) = (if z =d x then @g u else x).
+Lemma walkupI_eq : forall u x, @g (walkupI u x) = (if z == x then @g u else x).
 Proof.
-move=> u x; rewrite /walkupI; case: (subdIoptP (setC1 z) x) => [v Hx Dv|Hx].
+move=> u x; rewrite /walkupI; case: (subdIoptP (predC1 z) x) => [v Hx Dv|Hx].
   by rewrite (negbE Hx).
 by rewrite (negbE2 Hx).
 Qed.
 
-Lemma walkup_seq : forall p : seq g, setC p z -> {q : seq g' | p = maps (@g) q}.
+Lemma walkup_seq : forall p : seq g, predC p z -> {q : seq g' | p = maps (@g) q}.
 Proof.
-elim=> [|x p Hrec]; [ by exists (Seq0 walkupE) | rewrite /= /setU1 ].
+elim=> [|x p Hrec]; [ by exists (Seq0 walkupE) | rewrite /= /predU1 ].
 move/norP=> [Hx Hp]; rewrite eqd_sym in Hx.
 by case: (Hrec Hp) => [q Dp]; exists (Adds (@g' Hx) q); rewrite Dp.
 Qed.
 
 Lemma not_glink_fp : negb (glink z z) ->
-  and3 ((z =d edge z) = false) ((z =d node z) = false) ((z =d face z) = false).
+  and3 ((z == edge z) = false) ((z == node z) = false) ((z == face z) = false).
 Proof.
 case/norP; move=> Hez; move/norP=> [Hnz Hfz].
 by split; rewrite eqd_sym; apply negbE.
@@ -198,7 +193,7 @@ Qed.
 
 Lemma base_skip_edge : fun_base (@g) edge edge (seq2 (node (face z)) (node z)).
 Proof.
-move=> [x Hx] [y Hy]; rewrite /setC mem_seq2 /eqdf {2}/eqd /=.
+move=> [x Hx] [y Hy]; rewrite /predC mem_seq2 /eqdf {2}/eqd /=.
 move/norP=> [Hex Hfex] .
 rewrite (monic2F_eqd (monicF_sym (Eedge g))) in Hex.
 rewrite (monic2F_eqd (Enode g)) in Hfex.
@@ -208,7 +203,7 @@ Qed.
 Lemma glink_fp_skip_edge : glink z z -> skip_edge =1 skip (Iedge g).
 Proof.
 move=> H [x Hx]; apply: to_g_inj; move: H.
-rewrite /glink /relU /setU /eqdf /= /skip1 /skip_edge1 eqd_sym.
+rewrite /glink /relU /predU /eqdf /= /skip1 /skip_edge1 eqd_sym.
 case: (z =P edge z) => [Dz|_].
   by clear; rewrite Dz (inj_eqd (Iedge g)) (negbE Hx).
 case: (node z =P z) => [Dnz|_] Dfz.
@@ -220,16 +215,16 @@ Definition cross_edge := cedge z (node z).
 
 Let z_comp := closure clink (preimage (@g) (clink z)).
 
-Let z_barb := subset (clink z) (set1 z).
+Let z_barb := subset (clink z) (pred1 z).
 
-Remark z_barb_z : z_barb = and3b (z =d edge z) (z =d node z) (z =d face z).
+Remark z_barb_z : z_barb = and3b (z == edge z) (z == node z) (z == face z).
 Proof.
 apply/subsetP/and3P => [Hbz|[_ Hnz Hfz] x].
   have Hfz := Hbz _ (clinkF _); rewrite -{1}[z]Eedge in Hbz.
   have Hfez := Hbz _ (clinkN _); split; auto.
     by rewrite -(inj_eqd (Iface g)) -(eqP Hfz).
-  by rewrite {2}(eqP Hfez) Eedge set11.
-rewrite /clink /relU /setU /eqdf.
+  by rewrite {2}(eqP Hfez) Eedge eqxx.
+rewrite /clink /relU /predU /eqdf.
 by rewrite {1}(eqP Hnz) (finv_f (Inode g)) -(eqP Hfz) orbb.
 Qed.
 
@@ -246,7 +241,7 @@ move=> u v; move/connectP=> [p Hp <-] {v}.
 elim: p u Hp => [|v p Hrec] u /=; first by rewrite connect0.
 move/andP=> [Hu Hp]; apply: (connect_trans _ (Hrec _ Hp)).
 (case/clinkP: Hu; move/(congr1 to_g); rewrite /= /skip1) => [->|<-].
-  case Hnv: (z =d node (@g v)); last by exact (connect1 (clinkN _)).
+  case Hnv: (z == node (@g v)); last by exact (connect1 (clinkN _)).
   apply: (connect_trans (connect1 (clinkN _))).
   rewrite {1}(eqP Hnv); exact (connect1 (clinkN _)).
 case: (z =P face (@g u)) => [Dz|_];
@@ -256,14 +251,14 @@ Qed.
 
 Remark z_comp_preimage : z_comp =1 preimage (@g) (connect clink z).
 Proof.
-move=> v; apply/set0Pn/idP.
+move=> v; apply/pred0Pn/idP.
   case; move=> u; case/andP; rewrite /preimage Sclink; move=> Huv Hu.
   exact (connect_trans (connect1 Hu) (clink_at_g Huv)).
 case/connectP=> p0; case/shortenP=> [] [|x p] /= Hp Up _ Dv {p0}.
   by case/eqP: (z_to_g v); rewrite -Dv.
 move/andP: Hp => [Hu Hp]; case/andP: Up; rewrite -mem_adds.
 case/walkup_seq; case=> [|x' p'] //= [Dx Dp] _.
-exists x'; rewrite /setI /preimage /= -(Dx) Hu andbT.
+exists x'; rewrite /predI /preimage /= -(Dx) Hu andbT.
 apply: (etrans (Sclink walkupE _ _)); apply/connectP.
 exists p'; last by rewrite Dx Dp last_maps in Dv; exact (to_g_inj Dv).
 apply/(pathP x') => [i Hi]; apply clink_at_g'.
@@ -272,14 +267,14 @@ rewrite {1}[sub]lock /= -Dx -Dp -lock.
 by apply: ((pathP _) Hp); rewrite Dp size_maps.
 Qed.
 
-Remark z_barb_comp : z_barb = (n_comp clink z_comp =d 0).
+Remark z_barb_comp : z_barb = (n_comp clink z_comp == 0).
 Proof.
-apply/subsetP/set0P => [Hbz u|Hcz x Hx].
-  apply/andP; case; clear; case/set0Pn; move=> [x Hx]; move/andP=> [_ Hzx].
-  by rewrite /preimage /= in Hzx; rewrite /setC1 (Hbz _ Hzx) in Hx.
+apply/subsetP/pred0P => [Hbz u|Hcz x Hx].
+  apply/andP; case; clear; case/pred0Pn; move=> [x Hx]; move/andP=> [_ Hzx].
+  by rewrite /preimage /= in Hzx; rewrite /predC1 (Hbz _ Hzx) in Hx.
 apply/idPn => [Hv]; pose v := @g' Hv; pose u := root clink v.
-case/idP: (Hcz u); rewrite /setI {1}/u (roots_root (Sclink walkupE)).
-by apply/set0Pn; exists v; rewrite /setI Sclink /u connect_root.
+case/idP: (Hcz u); rewrite /predI {1}/u (roots_root (Sclink walkupE)).
+by apply/pred0Pn; exists v; rewrite /predI Sclink /u connect_root.
 Qed.
 
 Let disconnected := 1 < n_comp clink z_comp.
@@ -289,13 +284,13 @@ Let n_comp_z disc := if glink z z then S z_barb else negb disc : nat.
 Remark not_cross_edge_walkup : negb cross_edge -> forall u v,
  @g u = edge z -> @g v = node (face z) -> cedge u v.
 Proof.
-move=> Hznz u v Du Dv; case Hez: (z =d edge z).
+move=> Hznz u v Du Dv; case Hez: (z == edge z).
   by case: u Du => [ez Hez'] Dez; rewrite -Dez /= (negbE Hez') in Hez.
   case/connectP: (etrans (Sedge g _ _) (fconnect1 _ z)).
 move=> p0; case/shortenP=> [p Hp Up _ {p0}] Dz.
 elim/last_ind: p Dz Up Hp => [|p z'] Dz; first by case/eqP: Hez.
 rewrite last_add_last -cats1 -cat_adds uniq_cat path_cat /= !andbT orbF.
-move=> Dz'; rewrite {z'}Dz' /setU1 eqd_sym Hez /= -uniq_adds.
+move=> Dz'; rewrite {z'}Dz' /predU1 eqd_sym Hez /= -uniq_adds.
 rewrite {2}/eqdf (monic2F_eqd (Eedge g)) -Dv -Du.
 move/andP=> [Up Hpz]; move/andP=> [Hp Ev].
 case: {Hpz}(walkup_seq Hpz) => [p' Dp]; apply/connectP.
@@ -312,13 +307,13 @@ Remark disconnected_cross_edge : disconnected -> negb (glink z z) /\ cross_edge.
 Proof.
 move=> Hdz; apply: andP; apply/idPn => [Hgze].
 have Huw: forall u w, node (@g u) = z -> face z = @g w -> connect clink u w.
-  move=> u w Du Dw; case Hez: (z =d edge z).
+  move=> u w Du Dw; case Hez: (z == edge z).
     apply eq_connect0; apply to_g_inj; apply Inode.
     by rewrite -Dw (eqP Hez) Eedge.
-  case Hnz: (z =d node z).
+  case Hnz: (z == node z).
     by rewrite -{1}Du (inj_eqd (Inode g)) eqd_sym z_to_g in Hnz.
-  case Hfz: (z =d face z); first by rewrite Dw z_to_g in Hfz.
-  rewrite /glink /relU /setU /eqdf -!(eqd_sym z) Hez Hnz Hfz /= in Hgze.
+  case Hfz: (z == face z); first by rewrite Dw z_to_g in Hfz.
+  rewrite /glink /relU /predU /eqdf -!(eqd_sym z) Hez Hnz Hfz /= in Hgze.
   apply: (connect_trans _ (connect1 (clinkN _))).
   pose v := @g' (negbI Hez); apply connect_trans with v.
     rewrite Sclink; apply connect1; apply/clinkP; right.
@@ -330,13 +325,13 @@ have Huw: forall u w, node (@g u) = z -> face z = @g w -> connect clink u w.
   by rewrite -(monic2F_eqd (Eedge g)) eqd_sym Hez.
 rewrite /disconnected ltnNge leq_eqVlt ltnS leqn0 -z_barb_comp orbC in Hdz.
 case/idP: Hdz {Hgze}; case Hbz: z_barb; [ done | apply/eqP ].
-case/set0Pn: Hbz => [x]; move/andP=> [Hzx Hx]; set u := @g' Hx.
-rewrite -(@eq_n_comp_r _ (closure clink (set2 u u))).
+case/pred0Pn: Hbz => [x]; move/andP=> [Hzx Hx]; pred u := @g' Hx.
+rewrite -(@eq_n_comp_r _ (closure clink (pred2 u u))).
   by rewrite (n_comp_closure2 (Sclink walkupE)) connect0.
-move=> v; apply/set0Pn/set0Pn; case=> [w]; move/andP=> [Hvw Dw].
-  exists w; rewrite /set2 orbb in Dw.
-  by rewrite /setI Hvw /preimage -((u =P w) Dw).
-exists u; rewrite /setI /set2 orbb set11 andbT; apply: (connect_trans Hvw).
+move=> v; apply/pred0Pn/pred0Pn; case=> [w]; move/andP=> [Hvw Dw].
+  exists w; rewrite /pred2 orbb in Dw.
+  by rewrite /predI Hvw /preimage -((u =P w) Dw).
+exists u; rewrite /predI /pred2 orbb eqxx andbT; apply: (connect_trans Hvw).
 case/clinkP: Dw; case/clinkP: Hzx; move=> Dx Dw; auto.
 - by apply eq_connect0; apply to_g_inj; apply Inode; rewrite -Dw.
 - by rewrite Sclink; auto.
@@ -345,17 +340,17 @@ Qed.
 
 Let ae x := has (cedge x) (seq2 z (node z)).
 
-Remark Hae : fclosed edge (setC ae).
-Proof. by move=> x y; move/eqP=> <-; rewrite /setC /ae /= -!cedge1. Qed.
+Remark Hae : fclosed edge (predC ae).
+Proof. by move=> x y; move/eqP=> <-; rewrite /predC /ae /= -!cedge1. Qed.
 
-Remark adj_ae : fun_adjunction (@g) edge edge (setC ae).
+Remark adj_ae : fun_adjunction (@g) edge edge (predC ae).
 Proof.
 apply: (strict_adjunction (Sedge walkupE) Hae to_g_inj).
   apply/subsetP => x Haex.
-  case Hx: (z =d x); last by exact (codom_f _ (@g' (negbI Hx))).
-  by rewrite -(eqP Hx) /setC /ae /= connect0 in Haex.
+  case Hx: (z == x); last by exact (codom_f _ (@g' (negbI Hx))).
+  by rewrite -(eqP Hx) /predC /ae /= connect0 in Haex.
 move=> [x Hx] [y Hy]; move/negbE2=> Haex; apply: {y Hy}base_skip_edge.
-rewrite /setC mem_seq2 /=; apply/orP=> [Dx]; case/orP: Haex.
+rewrite /predC mem_seq2 /=; apply/orP=> [Dx]; case/orP: Haex.
 rewrite /seq1 /=; case: Dx; move/eqP=> <- {x Hx}.
   by left; rewrite cedge1 Eface connect0.
 by right; rewrite connect0.
@@ -368,14 +363,14 @@ Proof. by case adj_ae; auto. Qed.
 Lemma sub_cskip_edge : negb cross_edge -> forall u v,
   cedge (@g u) (@g v) -> cedge u v.
 Proof.
-move=> Hz u v Huv; case Hez: (z =d edge z).
+move=> Hz u v Huv; case Hez: (z == edge z).
   apply: (etrans (eq_fconnect (glink_fp_skip_edge _) _ _)).
     by apply/orP; left; rewrite eqd_sym in Hez.
   by rewrite fconnect_skip.
 case/connectP: Huv => [p].
 elim: {p}(S (size p)) {-2}p u (ltnSn (size p)) => [|n Hrec] //.
 move=> [|y p] u /= Hn; first by move=> *; apply eq_connect0; apply to_g_inj.
- move/andP=> [Dy Hp] Ep; case Hy: (z =d y).
+ move/andP=> [Dy Hp] Ep; case Hy: (z == y).
   case: p => [|ez p] /= in Hn Hp Ep |- *; first by rewrite Ep z_to_g in Hy.
   case/andP: Hp => [Dez Hp].
   have Eu: @g u = node (face z) by rewrite (eqP Hy) -(eqP Dy) Eedge.
@@ -384,15 +379,15 @@ move=> [|y p] u /= Hn; first by move=> *; apply eq_connect0; apply to_g_inj.
   move: Hp Ep; rewrite -(eqP Dez) -(eqP Hy) -{1 2}Eu'.
   exact: Hrec (ltnW Hn).
 apply: connect_trans (Hrec _ (@g' (negbI Hy)) Hn Hp Ep).
-case Hfy: (z =d face y).
+case Hfy: (z == face y).
   have Eeu: @g (edge u) = edge z by rewrite /= /skip_edge1 Hez (eqP Dy) Hfy.
-  have Hnfz: (negb (z =d node (face z))).
+  have Hnfz: (negb (z == node (face z))).
     by rewrite -(monic2F_eqd (Eedge g)) eqd_sym Hez.
   rewrite cedge1; pose u' := @g' Hnfz.
   apply: (connect_trans (@not_cross_edge_walkup _ _ u' _ _)); auto.
-  apply: connect1; rewrite /eqdf /eqd /= /skip_edge1 Hez Eface set11.
-  by rewrite {1 4}(eqP Hfy) Eface (inj_eqd (Iface g)) (eqd_sym y) Hy set11.
-by apply connect1; rewrite /eqdf /eqd /= /skip_edge1 Hez (eqP Dy) Hfy Hy set11.
+  apply: connect1; rewrite /eqdf /eqd /= /skip_edge1 Hez Eface eqxx.
+  by rewrite {1 4}(eqP Hfy) Eface (inj_eqd (Iface g)) (eqd_sym y) Hy eqxx.
+by apply connect1; rewrite /eqdf /eqd /= /skip_edge1 Hez (eqP Dy) Hfy Hy eqxx.
 Qed.
 
 Lemma cskip_edge_merge : negb cross_edge ->
@@ -403,15 +398,15 @@ move=> Hz u v Hu; apply/idP/idP => [Huv|].
   rewrite Sedge (same_cskip_edge Hv) Sedge in Huv.
   exact (etrans (closed_connect Hae Huv) Hv).
 move: Hu; rewrite /ae /= !orbF.
-case Hez: (z =d (edge z)).
+case Hez: (z == (edge z)).
   have Hzz: fcycle edge (seq1 z) by rewrite /= /eqdf eqd_sym Hez.
-  rewrite -!(Sedge g z) !(fconnect_cycle Hzz (setU11 _ _)) /= /setU1 !z_to_g.
+  rewrite -!(Sedge g z) !(fconnect_cycle Hzz (predU11 _ _)) /= /predU1 !z_to_g.
   by move=> Hu Hv; apply (sub_cskip_edge Hz); rewrite (same_cedge Hu) Sedge.
 have Hnfz := Hez; rewrite eqd_sym (monic2F_eqd (Eedge g)) in Hnfz.
 pose uez := @g' (negbI Hez); pose unfz := @g' (negbI Hnfz).
 have Henz := (@not_cross_edge_walkup Hz uez unfz (erefl _) (erefl _)).
 rewrite cedge1r in Henz; have Eenz: @g (edge unfz) = edge (node z).
-  rewrite /= /skip_edge1 Hez Eface set11.
+  rewrite /= /skip_edge1 Hez Eface eqxx.
   case: (z =P face z) => [Dfz|_] //; case/idP: Hz.
   by rewrite /cross_edge -{1}[z]Eface -Dfz Sedge fconnect1.
 case/orP=> [Hu|Hu]; case/orP=> [Hv|Hv];
@@ -426,7 +421,7 @@ by rewrite /= -cedge1 Sedge.
 Qed.
 
 Remark fcard_skip_edge :
-  let Sez := if glink z z then S (z =d edge z) else double (negb cross_edge) in
+  let Sez := if glink z z then S (z == edge z) else double (negb cross_edge) in
   Sez + (fcard edge g') = S (fcard edge g).
 Proof.
 case Hgzz: (glink z z).
@@ -438,47 +433,47 @@ pose unfz := @g' (negbI Hnfz); pose unz := @g' (negbI Hnz).
 have Heg := Sedge g; have Heg' := (Sedge g').
 rewrite (n_compC ae) (n_compC (preimage (@g) ae)).
 rewrite (adjunction_n_comp _ Heg Heg' Hae adj_ae) -addSn !addnA; congr addn.
-have Eae: ae =1 fclosure edge (set2 z (node z)).
-  move=> x; rewrite /ae /= orbF; apply/orP/set0Pn; case.
-  - by exists z; rewrite /setI /set2 set11 /= andbT.
-  - by exists (node z); rewrite /setI /set2 set11 orbT andbT.
+have Eae: ae =1 fclosure edge (pred2 z (node z)).
+  move=> x; rewrite /ae /= orbF; apply/orP/pred0Pn; case.
+  - by exists z; rewrite /predI /pred2 eqxx /= andbT.
+  - by exists (node z); rewrite /predI /pred2 eqxx orbT andbT.
   move=> y; case/andP=> [Hxy].
   by case/orP; move/eqP=> Dy; rewrite -Dy in Hxy; auto.
 rewrite (eq_n_comp_r Eae) (n_comp_closure2 Heg).
-have Hag': preimage (@g) ae =1 fclosure edge (set2 unfz unz).
-  move=> u; rewrite /preimage /ae /= orbF; apply/idP/set0Pn => [Hu|[v Hv]].
-    have [y Huy Hy]: exists2 y, cedge (@g u) y & set2 (@g unfz) (@g unz) y.
-      rewrite /set2 /=; case/orP: Hu.
-        by exists (node (face z)); [ rewrite cedge1r Eface | rewrite set11 ].
-      by exists (node z); last by rewrite set11 orbT.
+have Hag': preimage (@g) ae =1 fclosure edge (pred2 unfz unz).
+  move=> u; rewrite /preimage /ae /= orbF; apply/idP/pred0Pn => [Hu|[v Hv]].
+    have [y Huy Hy]: exists2 y, cedge (@g u) y & pred2 (@g unfz) (@g unz) y.
+      rewrite /pred2 /=; case/orP: Hu.
+        by exists (node (face z)); [ rewrite cedge1r Eface | rewrite eqxx ].
+      by exists (node z); last by rewrite eqxx orbT.
     move/connectP: Huy Hy {Hu} => [p Hp <-] {y}.
-    elim: p u Hp => [|y p Hrec] u /=; first by exists u; rewrite /setI connect0.
-    move/andP=> [Dy Hp]; case Hex: (z =d edge (@g u)).
-      exists u; rewrite /setI connect0 /set2 /eqd /= {1}(eqP Hex) Eedge.
-      by rewrite /to_g set11.
-    case Hfex: (z =d face (edge (@g u))).
-      exists u; rewrite /setI connect0 /set2 /eqd /= {3}(eqP Hfex) Eedge.
-      by rewrite /to_g set11 orbT.
-    have Hu': setC1 z y by rewrite /setC1 -(eqP Dy) Hex.
+    elim: p u Hp => [|y p Hrec] u /=; first by exists u; rewrite /predI connect0.
+    move/andP=> [Dy Hp]; case Hex: (z == edge (@g u)).
+      exists u; rewrite /predI connect0 /pred2 /eqd /= {1}(eqP Hex) Eedge.
+      by rewrite /to_g eqxx.
+    case Hfex: (z == face (edge (@g u))).
+      exists u; rewrite /predI connect0 /pred2 /eqd /= {3}(eqP Hfex) Eedge.
+      by rewrite /to_g eqxx orbT.
+    have Hu': predC1 z y by rewrite /predC1 -(eqP Dy) Hex.
     case/(Hrec (@g' Hu') Hp) {Hrec} => v; move/andP=> [Hu'v Dv].
-    exists v; simpl in Dv; rewrite /setI Dv andbT.
+    exists v; simpl in Dv; rewrite /predI Dv andbT.
     apply: (connect_trans (connect1 _) Hu'v).
     by rewrite /eqdf /eqd /= /skip_edge1 Hez -/to_g Hex Hfex.
   case/andP: Hv; move/connectP=> [p Hp <-] {v}.
   elim: p u Hp => [|v p Hrec] [x Hx] /=.
-    rewrite {1}/set2 /eqd /=; clear; case/orP; move/eqP=> Dx.
+    rewrite {1}/pred2 /eqd /=; clear; case/orP; move/eqP=> Dx.
       by rewrite -Dx cedge1 Eface connect0.
     by rewrite Dx connect0 orbT.
   move=> H Ep; case/andP: H; rewrite {1}/eqdf /eqd /= /skip_edge1 Hez.
-  case Hex: (z =d edge x); first by do 2 clear; rewrite (eqP Hex) fconnect1.
-  case Hfex: (z =d face (edge x)).
+  case Hex: (z == edge x); first by do 2 clear; rewrite (eqP Hex) fconnect1.
+  case Hfex: (z == face (edge x)).
     by do 2 clear; rewrite (eqP Hfex) Eedge connect0 orbT.
   move=> Dex Hp; rewrite !(cedge1 x) (eqP Dex); exact (Hrec _ Hp Ep).
 rewrite (eq_n_comp_r Hag') (n_comp_closure2 Heg') -/cross_edge.
 case Hznz: cross_edge; rewrite /cross_edge in Hznz.
   rewrite -{1}[z]Eface -cedge1 in Hznz; case/connectP: Hznz => q.
   case/shortenP=> [[|z' p] Hp Up _ {q}] /= Dnfz.
-    by rewrite (Inode _ Dnfz) set11 in Hfz.
+    by rewrite (Inode _ Dnfz) eqxx in Hfz.
   rewrite /= {1}/eqdf Eface in Hp; case/andP: Hp => Dz'.
   move/eqP: Dz' Up Dnfz => <- {z'} /=; case/and3P.
   move/norP=> [_ Hpnfz] Hpz Up Dnz Hp.
@@ -486,7 +481,7 @@ case Hznz: cross_edge; rewrite /cross_edge in Hznz.
     by rewrite Dp in Dnz; case/eqP: (Hnz).
   rewrite Dp /= in Hp; move/andP: Hp => [Dez Hp].
   have Hunz: eqdf edge unz uez.
-    by rewrite /eqdf /eqd /= -/to_g /skip_edge1 -(eqP Dez) Hez Enode !set11.
+    by rewrite /eqdf /eqd /= -/to_g /skip_edge1 -(eqP Dez) Hez Enode !eqxx.
   have Dunz: unz = last uez p'.
     by apply: to_g_inj; rewrite -last_maps /= -Dnz Dp.
   have Hp': fcycle edge (Adds uez p').
@@ -500,14 +495,14 @@ case Hznz: cross_edge; rewrite /cross_edge in Hznz.
   by rewrite Dp /= in Hpnfz; rewrite -(mem_maps to_g_inj) /= Hpnfz.
 have Hw: cedge unfz unz; last by rewrite Hw.
 rewrite Heg' cedge1; apply: (not_cross_edge_walkup (negbI Hznz)); last done.
-by rewrite /= /skip_edge1 Hez Enode set11.
+by rewrite /= /skip_edge1 Hez Enode eqxx.
 Qed.
 
 Lemma base_clink_walkup :
   rel_base (@g) clink clink (seq2 (edge (node z)) (node z)).
 Proof.
-move=> [x Hx] [y Hy]; rewrite /setC mem_seq2 /=; move/norP=> [Hex Hfex].
-rewrite /clink /relU /setU /eqdf !(monic2F_eqd (f_finv (Inode _))) /=.
+move=> [x Hx] [y Hy]; rewrite /predC mem_seq2 /=; move/norP=> [Hex Hfex].
+rewrite /clink /relU /predU /eqdf !(monic2F_eqd (f_finv (Inode _))) /=.
 rewrite {3 4}/eqd /= /skip1 -(monic2F_eqd (monicF_sym (Eface g))) (negbE Hex).
 by case: (z =P node y) => [<-|_] //; rewrite !(eqd_sym x) (negbE Hfex) (negbE Hx).
 Qed.
@@ -523,14 +518,14 @@ Remark n_comp_glink_walkup :
 Proof.
 have Hsg := (Sclink g); have Hsg' := (Sclink g').
 pose a := connect clink z.
-have Ha: closed clink (setC a) by apply: setC_closed; apply: connect_closed.
-have Haa: rel_adjunction (@g) clink clink (setC a).
+have Ha: closed clink (predC a) by apply: predC_closed; apply: connect_closed.
+have Haa: rel_adjunction (@g) clink clink (predC a).
   apply (strict_adjunction Hsg' Ha to_g_inj).
-    apply/subsetP => [x Hax]; case Hx: (z =d x).
-      by rewrite /setC /a -(eqP Hx) connect0 in Hax.
+    apply/subsetP => [x Hax]; case Hx: (z == x).
+      by rewrite /predC /a -(eqP Hx) connect0 in Hax.
     exact (codom_f (@g) (@g' (negbI Hx))).
   move=> [x Hx] v; move/negbE2=> Hax; simpl in Hax; apply: {v}base_clink_walkup.
-  rewrite /setC mem_seq2 /= {Hx}; apply/orP => Dx; case/idP: Hax.
+  rewrite /predC mem_seq2 /= {Hx}; apply/orP => Dx; case/idP: Hax.
   case: Dx; case/eqP=> <- {x}; rewrite /a Hsg.
     rewrite -{2}[z]Enode; apply connect1; apply clinkF.
   apply connect1; apply clinkN.
@@ -543,16 +538,16 @@ case: (not_glink_fp Hgzz) => [_ Hfez Hfz].
   rewrite eqd_sym (monic2F_eqd (Enode g)) in Hfez.
   apply: eqP; rewrite /= add0n eqn_leq; apply/andP; split; last by exact Hdz.
   pose u := @g' (negbI Hfez); pose v := @g' (negbI Hfz).
-  rewrite -(@eq_n_comp_r _ (closure clink (set2 u v))).
+  rewrite -(@eq_n_comp_r _ (closure clink (pred2 u v))).
     by rewrite n_comp_closure2; case (connect clink u v).
   move=> w; rewrite /z_comp /closure !(disjoint_sym (connect clink w)).
   congr negb; apply: {w}eq_disjoint => w; apply/orP/clinkP.
     by move=> [Dw|Dw]; [ left | right ]; rewrite -((_ =P w) Dw) /= ?Eedge.
   rewrite /eqd /= -/to_g.
-  by move=> [Dz|<-]; [ left; rewrite Dz | right ]; rewrite ?Enode set11.
+  by move=> [Dz|<-]; [ left; rewrite Dz | right ]; rewrite ?Enode eqxx.
 move: (negbI Hdz); rewrite /disconnected -leqNgt leq_eqVlt ltnS leqn0.
 rewrite -z_barb_comp orbC; case Hbz: z_barb.
-have Hez: z =d edge z by rewrite z_barb_z in Hbz; case (andP Hbz).
+have Hez: z == edge z by rewrite z_barb_z in Hbz; case (andP Hbz).
 rewrite {2}(eqP Hez) glinkE; rewrite z_barb_comp in Hbz.
   by rewrite (eqP Hbz).
 by simpl; move/eqP=> ->; rewrite if_same.
@@ -571,11 +566,11 @@ Proof.
 rewrite /genus_rhs -(fcard_skip (Inode g)) -(fcard_skip (Iface g)).
 rewrite -addSn -fcard_skip_edge addnC -!addnA; symmetry.
 do 3 (rewrite addnC -!addnA; congr addn).
-rewrite /n_comp_z /glink /relU /setU /eqdf -!(eqd_sym z) z_barb_z.
-case Hnz: (z =d node z).
+rewrite /n_comp_z /glink /relU /predU /eqdf -!(eqd_sym z) z_barb_z.
+case Hnz: (z == node z).
   rewrite -(eqd_sym (face z)) (monic2F_eqd (Eface g)) -(eqP Hnz).
-  by case (z =d edge z).
-case Hfz: (z =d face z); last by case (z =d edge z).
+  by case (z == edge z).
+case Hfz: (z == face z); last by case (z == edge z).
 by rewrite -(eqd_sym (edge z)) (monic2F_eqd (Eedge g)) -(eqP Hfz) Hnz.
 Qed.
 
@@ -612,7 +607,7 @@ by case: (disconnected_cross_edge Hdz) => [_ Hznz]; rewrite Hznz.
 Qed.
 
 Definition skip_clink : rel g :=
-  fun x y => (x =d skip1 node y) || (skip1 face x =d y).
+  fun x y => (x == skip1 node y) || (skip1 face x == y).
 
 Lemma skip_clink_walkup : forall x' p',
   path clink x' p' = path skip_clink (@g x') (maps (@g) p').
@@ -621,11 +616,11 @@ move=> x' p'; elim: p' x' => [|y' p' Hrec] x' //=; rewrite {}Hrec.
 by congr andb; congr orb; rewrite /eqdf (monic2F_eqd (f_finv (Inode walkupE))).
 Qed.
 
-Lemma skip_clinkf : forall x y, skip_clink x y -> negb (x =d node z) ->
+Lemma skip_clinkf : forall x y, skip_clink x y -> negb (x == node z) ->
  clink x y \/ face x = z /\ face z = y.
 Proof.
 move=> x y Hxy' Hxnz; case: {Hxy'}(orP Hxy'); rewrite /skip1.
-  case (z =d node y); move=> Dx; first by rewrite Dx in Hxnz.
+  case (z == node y); move=> Dx; first by rewrite Dx in Hxnz.
   by left; rewrite (eqP Dx) clinkN.
 case: (z =P face x) => [Dfx|_] Dfy.
   by right; split; last by exact (eqP Dfy).
@@ -666,13 +661,13 @@ have Hynx: mem2 p' y (skip1 node x).
   by rewrite -(mem2_maps to_g_inj) in Hynu.
 have Ep: skip1 node y = last x p'.
   rewrite /p' /x last_maps; exact (congr1 (@g) (f_finv (Inode _) (last u pw))).
-case Hxy: (x =d y); first by rewrite /p (eqP Hxy) /= (mem2l Hynx) in Up.
-have Hzy: (z =d y) = false by apply: z_to_g.
+case Hxy: (x == y); first by rewrite /p (eqP Hxy) /= (mem2l Hynx) in Up.
+have Hzy: (z == y) = false by apply: z_to_g.
 clearbody p' x y; move: {pw Upw Hynu}Ep Hynx; rewrite /skip1.
 case Hpnz: (negb (p (node z))).
-  case: (z =d node y); first by move=> Dnz; rewrite /p Dnz mem_last in Hpnz.
-  case: (z =d node x) => [|] Ep Hynx.
-    by rewrite /p /= (setU1r x (mem2r Hynx)) in Hpnz.
+  case: (z == node y); first by move=> Dnz; rewrite /p Dnz mem_last in Hpnz.
+  case: (z == node x) => [|] Ep Hynx.
+    by rewrite /p /= (predU1r x (mem2r Hynx)) in Hpnz.
   case: {Hpw}(splice_face_clink Hpw Up).
   + by apply/idP => [Hnz]; case/idP: Hpnz; apply: mem_belast.
   + by move=> Hp; case/and3P: (Hj p); split; rewrite // -Ep Einng.
@@ -701,8 +696,8 @@ case: {Hpw}(splice_face_clink Hpw Up).
     + by rewrite -cats1 -cat_adds Dp uniq_cat Up /= orbF Hpz.
     by rewrite -cats1 path_cat Ep Hp /= clinkN.
   rewrite /= Ep; move/andP=> [Dfez Hqw] Hp.
-  case Hzfez: (z =d fez); first by rewrite Dq (eqP Hzfez) /= setU11 in Hqz.
-  case: (z =d node y) => [|] Eq; first by rewrite Dq Eq mem_last in Hqnz.
+  case Hzfez: (z == fez); first by rewrite Dq (eqP Hzfez) /= predU11 in Hqz.
+  case: (z == node y) => [|] Eq; first by rewrite Dq Eq mem_last in Hqnz.
   rewrite Dq in Uq; case: {Hqw}(splice_face_clink Hqw Uq).
   + by apply/idP => H; case/idP: Hqnz; rewrite Dq mem_belast.
   + move=> Hq Hynx; rewrite -Dq in Uq; case Hzq: (clink z fez).
@@ -710,18 +705,18 @@ case: {Hpw}(splice_face_clink Hpw Up).
       * rewrite last_cat {2}Dq /= -Eq Einng.
         case: (z =P node x) Hynx => [Dz|_] Hynx; last by apply mem2_splice1.
         rewrite (mem2r_cat Hqnz) in Hynx.
-        by rewrite -Dz mem2_cat /= setU11 (mem2l Hynx) orbC.
+        by rewrite -Dz mem2_cat /= predU11 (mem2l Hynx) orbC.
       * by rewrite -cat_adds Dp uniq_cat Up /= negb_orb Upq Hpz Hqz.
       by rewrite path_cat Hp Dq /= Ep clinkN Hzq.
     case/orP: Dfez; rewrite /skip1.
       case: (z =P node fez) => [Dz|_] Dnz; first by rewrite Dz clinkN in Hzq.
-      by rewrite (Inode g (eqP Dnz)) Dq /= setU11 in Hqz.
-    case: (z =d face (node z)) => [|] Dfez.
+      by rewrite (Inode g (eqP Dnz)) Dq /= predU11 in Hqz.
+    case: (z == face (node z)) => [|] Dfez.
       by rewrite -(eqP Dfez) clinkF in Hzq.
     case: (z =P node x) Hynx => [Dz|_] Hynx.
       case/and3P: (Hj (Adds z (Adds x (cat p' q)))); split.
       * by rewrite /= last_cat {2}Dq /= -Eq Einng mem2_adds Hxy.
-      * rewrite -cat_adds Dp /= uniq_cat Up Upq mem_cat /setU negb_orb.
+      * rewrite -cat_adds Dp /= uniq_cat Up Upq mem_cat /predU negb_orb.
         by rewrite Hqz Hpz.
       rewrite Dq /= {1}Dz path_cat clinkN Hp Ep /=.
       by rewrite -{1}(eqP Dfez) clinkF.
@@ -737,17 +732,17 @@ case: {Hpw}(splice_face_clink Hpw Up).
   rewrite Dq has_cat in Upq; case/norP: Upq => [Upq1 Upq2].
   case/orP: Dfez; rewrite Dq /skip1.
     case: (z =P node fez) {q Dq Hqnz} => [Dz|_] Dnz;
-      last by rewrite (Inode g (eqP Dnz)) -Dq1 /= setU11 in Hq1z.
+      last by rewrite (Inode g (eqP Dnz)) -Dq1 /= predU11 in Hq1z.
     case: (z =P node x) {Dnz} => [Dz'|_] Hynx.
-      case/hasP: Upq1; exists fez; first by rewrite -Dq1 /= setU11.
-      by rewrite Dz in Dz'; rewrite (Inode g Dz') -Dp /= setU11.
+      case/hasP: Upq1; exists fez; first by rewrite -Dq1 /= predU11.
+      by rewrite Dz in Dz'; rewrite (Inode g Dz') -Dp /= predU11.
     case Hq1y: (q1 y).
       case/and3P: (Hj (Adds fez (cat q1' (Adds z q2)))); split.
       + rewrite last_cat -{2}Dq2 /= -Eq2 Einng -Dz.
         rewrite -Dq1 /= in Hq1y; case/orP: Hq1y.
         rewrite -(inj_eqd (Inode g)) Eq2 -Dz; move/eqP=> Eq2'.
         by rewrite Eq2' -Dq2 mem_last in Hq2z.
-      + by move=> Hq1'y; rewrite mem2_cat Hq1'y /= setU11 /= orbT.
+      + by move=> Hq1'y; rewrite mem2_cat Hq1'y /= predU11 /= orbT.
       + by rewrite -cat_adds Dq1 uniq_cat Uq1 /= negb_orb Hq1z Uq12 Hq2z.
       by rewrite path_cat Hq1 -Dq2 /= -{1}Eq1 !clinkF.
     case Hq1nx: (q1 (node x)).
@@ -765,8 +760,8 @@ case: {Hpw}(splice_face_clink Hpw Up).
       case/and3P: (Hj (Adds fez (cat q3' (cat p (Adds z q2))))); split.
       + rewrite catA last_cat -{2}Dq2 /= -Eq2 Einng -Dz mem2_cat /=.
         apply/orP; right; move: (mem2l Hynx).
-        rewrite !mem_cat /setU (negbE Hq3y) orbF orbC.
-        by move=> Hpy; rewrite -Dp /= (setU1r x Hpy) setU11.
+        rewrite !mem_cat /predU (negbE Hq3y) orbF orbC.
+        by move=> Hpy; rewrite -Dp /= (predU1r x Hpy) predU11.
       + rewrite -cat_adds Dq3 !uniq_cat Uq3 Up has_cat /= !negb_orb Upq2.
         by rewrite !(has_sym q3) Upq3 Uq23 Hq3z Hpz Hq2z.
       by rewrite !path_cat Hq3 Eq3 -Dp -Dq2 /= Hp Ep !clinkN clinkF.
@@ -781,8 +776,8 @@ case: {Hpw}(splice_face_clink Hpw Up).
   case/and3P: (Hj (Adds x (cat p' (cat q1 (Adds z q2))))); split.
   + rewrite catA last_cat -{2}Dq2 /= -Eq2 Einng.
     case: (z =P node x) Hynx => [Dz|_].
-      rewrite -Dz -Dq (mem2r_cat Hqnz) mem2_cat /= setU11 orbC.
-      by move=> Hpy; rewrite mem_cat /setU (mem2l Hpy).
+      rewrite -Dz -Dq (mem2r_cat Hqnz) mem2_cat /= predU11 orbC.
+      by move=> Hpy; rewrite mem_cat /predU (mem2l Hpy).
     by rewrite catA; apply: mem2_splice1.
   + rewrite -cat_adds Dp !uniq_cat has_cat /= !negb_orb.
     by rewrite Up Upq1 Hpz Upq2 Uq1 Hq1z Uq12 Hq2z.
@@ -793,9 +788,9 @@ move Dp1: (Adds x p1') => p1; move Dp2: (Adds (face z) p2') => p2 Dp.
 rewrite -Dp uniq_cat in Up; case/and3P: Up => [Up1 Up12 Up2].
 rewrite -Dp has_sym has_cat in Upq; case/norP: Upq => [Uqp1 Uqp2].
 rewrite -Dp mem_cat in Hpz; case/norP: Hpz => [Hp1z Hp2z].
-case Hp2nx: (setU1 z p2 (node x)).
+case Hp2nx: (predU1 z p2 (node x)).
   case/and3P: (Hj (Adds x (cat p1' (Adds z p2)))); split.
-  - rewrite last_cat -{2}Dp2 /= Ep2 Einng mem2_cat mem2_adds set11 Hp2nx.
+  - rewrite last_cat -{2}Dp2 /= Ep2 Einng mem2_cat mem2_adds eqxx Hp2nx.
     by rewrite orbT.
   - by rewrite -cat_adds Dp1 uniq_cat /= negb_orb Up1 Hp1z Up12 Hp2z.
   by rewrite path_cat Hp1 -Dp2 /= -{1}Ep1 !clinkF.
@@ -808,16 +803,16 @@ case Dq: {1 2}q Hqw => [|fez q'] /=.
   - by rewrite last_add_last {2}Dz Einng -cats1 mem2_cat Hynx.
   - by rewrite -cats1 -cat_adds Dp1 uniq_cat /= Up1 orbF andbT.
   by rewrite -cats1 path_cat Hp1 /= -Ep1 clinkF.
-case: (z =d (node y)); first by move=> _ Dnz; rewrite Dnz Dq mem_last in Hqnz.
+case: (z == (node y)); first by move=> _ Dnz; rewrite Dnz Dq mem_last in Hqnz.
 move/andP=> [Dfez Hqw] Eq Hynx; have Uq' := Uq; rewrite Dq in Uq'.
 case: {Hqw Uq'}(splice_face_clink Hqw Uq').
 - by apply/idP => [Hnz]; case/idP: Hqnz; rewrite Dq mem_belast.
 - case/orP: Dfez {Hqnz}; rewrite /skip1.
     case: (z =P node fez) => [Dz|_] Dnz;
-      last by rewrite (Inode g (eqP Dnz)) Dq /= setU11 in Hqz.
+      last by rewrite (Inode g (eqP Dnz)) Dq /= predU11 in Hqz.
     case Hp2y: (p2 y) {Dnz} => [|] Hq.
       case Hp1y: (p1' y) {Hp2nx}.
-        by case/hasP: Up12; exists y; last by rewrite -Dp1 /= setU1r.
+        by case/hasP: Up12; exists y; last by rewrite -Dp1 /= predU1r.
       rewrite -Dp2 in Hp2y.
       case/splitPl: {p2'}Hp2y Ep2 Dp2 Hp2 => [p3' p4' Ep3].
       rewrite last_cat -cat_adds lastI path_cat {}Ep3 cat_add_last.
@@ -826,31 +821,31 @@ case: {Hqw Uq'}(splice_face_clink Hqw Uq').
       rewrite -Dp2 !has_cat uniq_cat mem_cat; move/norP=> [_ Up14].
       move/norP=> [_ Uqp4]; move/and3P=> [_ Up34 Up4]; move/norP=> [_ Hp4z].
       case Hp3y: (p3 y).
-        by case/hasP: Up34; exists y; first by rewrite -Dp4 /= setU11.
+        by case/hasP: Up34; exists y; first by rewrite -Dp4 /= predU11.
       rewrite -Dp2 -catA (mem2l_cat Hp1y) -catA (mem2l_cat Hp3y) in Hynx.
       case/and3P: (Hj (Adds x (cat p1' (cat (Adds z q) p4)))); split.
-      + rewrite !last_cat -{2}Dp4 /= Ep4 Einng mem2_cat mem2_adds set11.
-        rewrite orbC /setU1 !orbA; apply/orP; right.
-        by move: (mem2r Hynx); rewrite !mem_cat /setU orbC.
+      + rewrite !last_cat -{2}Dp4 /= Ep4 Einng mem2_cat mem2_adds eqxx.
+        rewrite orbC /predU1 !orbA; apply/orP; right.
+        by move: (mem2r Hynx); rewrite !mem_cat /predU orbC.
       + rewrite -cat_adds Dp1 uniq_cat Up1 /= uniq_cat has_cat Uq mem_cat.
-        by rewrite /setU !negb_orb Hp1z Hqz Hp4z Uqp4 Up14 has_sym Uqp1.
+        by rewrite /predU !negb_orb Hp1z Hqz Hp4z Uqp4 Up14 has_sym Uqp1.
       by rewrite !path_cat Hp1 Dq -Dp4 /= Hq -{1}Ep1 Dz -Eq !clinkN clinkF.
     rewrite (mem2lr_splice Hp2y (negbE Hp2nx)) in Hynx.
     case/and3P: (Hj (Adds x (cat p1' (Adds z q)))); split.
     + by rewrite last_cat {2}Dq /= -Eq Einng; apply mem2_splice1.
     + by rewrite -cat_adds Dp1 uniq_cat Up1 /= negb_orb Hp1z has_sym Uqp1 Hqz.
     by rewrite path_cat Hp1 Dq /= -{1}Ep1 clinkF Dz clinkN.
-  case: (z =d face (node z)) => [|] Dfz Hq.
-    case/hasP: Uqp2; exists fez; last by rewrite Dq /= setU11.
-    by rewrite -(eqP Dfz) -Dp2 /= setU11.
+  case: (z == face (node z)) => [|] Dfz Hq.
+    case/hasP: Uqp2; exists fez; last by rewrite Dq /= predU11.
+    by rewrite -(eqP Dfz) -Dp2 /= predU11.
   case/and3P: (Hj (Adds x (cat p1' (cat (Adds z p2) q)))); split.
   + by rewrite !last_cat {2}Dq /= -Eq Einng mem2_splice1 ?catA.
-  + rewrite -cat_adds Dp1 uniq_cat Up1 /= has_cat uniq_cat Up2 mem_cat /setU.
+  + rewrite -cat_adds Dp1 uniq_cat Up1 /= has_cat uniq_cat Up2 mem_cat /predU.
     by rewrite !negb_orb Hp1z Up12 has_sym Uqp1 Hqz Hp2z has_sym Uqp2.
   by rewrite !path_cat Hp1 -Dp2 Dq /= Hp2 Hq -{1}Ep1 Ep2 -(eqP Dfz) !clinkF.
 move=> [q1 _ [q2 _ Dq']]; case/hasP: Uqp2; exists (face z).
-  by rewrite -Dp2 /= setU11.
-by rewrite Dq -Dq' /= /setU1 mem_cat /setU /= setU11 !orbT.
+  by rewrite -Dp2 /= predU11.
+by rewrite Dq -Dq' /= /predU1 mem_cat /predU /= predU11 !orbT.
 Qed.
 
 End Walkup.
